theories/program_logic/traces.v
@@ -1,0 +1,191 @@
+From aneris.program_logic Require Export weakestpre.
+
+Set Default Proof Using "Type".
+Import uPred.
+
+Record execution_trace Λ := {
+  extr_confs : list (cfg Λ);
+  extr_obs : list (list (observation Λ)); }.
+
+Arguments extr_confs {_} _.
+Arguments extr_obs {_} _.
+
+Lemma app_singleton_inv {A} (e e' : list A) (x x' : A) :
+  e ++ [x] = e' ++ [x'] → e = e' ∧ x = x'.
+Proof.
+  rewrite -(reverse_involutive (e ++ [x])).
+  rewrite -(reverse_involutive (e' ++ [x'])).
+  intros Heq.
+  eapply (inj (R := (=))) in Heq; last apply _.
+  rewrite !reverse_app /= in Heq; simplify_eq; done.
+Qed.
+
+Section execution_trace.
+  Context {Λ : language}.
+
+  Definition singleton_exec (c : cfg Λ) : execution_trace Λ :=
+    {| extr_confs := [c]; extr_obs := []; |}.
+
+  Definition exec_starts_in (ex : execution_trace Λ) (c : cfg Λ) : Prop :=
+    hd_error (extr_confs ex) = Some c.
+
+  Definition exec_ends_in (ex : execution_trace Λ) (c : cfg Λ) : Prop :=
+    last (extr_confs ex) = Some c.
+
+  Lemma singleton_exec_starts_in c : exec_starts_in (singleton_exec c) c.
+  Proof. done. Qed.
+
+  Lemma singleton_exec_ends_in c : exec_ends_in (singleton_exec c) c.
+  Proof. done. Qed.
+
+  Lemma exec_ends_in_inj ex c c' :
+    exec_ends_in ex c → exec_ends_in ex c' → c = c'.
+  Proof. rewrite /exec_ends_in; intros ->; congruence. Qed.
+
+  Definition exec_extend (ex : execution_trace Λ)
+             (κ : list (observation Λ)) (c : cfg Λ) :=
+    {| extr_confs := extr_confs ex ++ [c];
+       extr_obs := extr_obs ex ++ [κ]; |}.
+
+  Definition exec_contract (ex ex' : execution_trace Λ) : Prop :=
+    ∃ c κ, ex = exec_extend ex' κ c.
+
+  Lemma exec_contract_of_extend ex κ c ex' :
+    exec_contract (exec_extend ex κ c) ex' → ex' = ex.
+  Proof.
+    rewrite /exec_contract /exec_extend.
+    destruct ex as [confs obs].
+    destruct ex' as [confs' obs'].
+    intros (? & ? & Heq); simplify_eq.
+    repeat match goal with
+             Heq : _ |- _ => apply app_singleton_inv in Heq as [? ?]
+           end; simplify_eq; done.
+  Qed.
+
+  Lemma not_exec_contract_singleton c ex :
+    ¬ exec_contract (singleton_exec c) ex.
+  Proof. intros (?&?&?); destruct ex as [? []]; simplify_eq. Qed.
+
+  Inductive valid_exec : execution_trace Λ → Prop :=
+  | valid_exec_singleton c : valid_exec (singleton_exec c)
+  | valid_exec_step ex c κ c' :
+      exec_ends_in ex c →
+      step c κ c' →
+      valid_exec ex →
+      valid_exec (exec_extend ex κ c').
+
+  Lemma valid_singleton_exec c : valid_exec (singleton_exec c).
+  Proof. constructor. Qed.
+
+  Lemma exec_extend_starts_in ex c' c κ :
+    exec_starts_in ex c' → exec_starts_in (exec_extend ex c κ) c'.
+  Proof.
+    rewrite /exec_starts_in /exec_extend /=; intros Hec'.
+    assert (extr_confs ex = c' :: tail (extr_confs ex)) as ->
+        by by apply hd_error_tl_repr.
+    done.
+  Qed.
+
+  Lemma exec_extend_ends_in ex c κ : exec_ends_in (exec_extend ex κ c) c.
+  Proof. apply last_snoc. Qed.
+
+  Lemma extend_valid_exec ex c κ c':
+    valid_exec ex →
+    exec_ends_in ex c →
+    step c κ c' →
+    valid_exec (exec_extend ex κ c').
+  Proof.
+    intros He; revert c κ c'.
+    induction He as [|? ? ? ? ? ? ? IHe]; intros c1 κ' c2.
+    - intros; econstructor; [done|done|constructor].
+    - intros; econstructor; [done|done|].
+      eapply IHe; eauto.
+  Qed.
+
+End execution_trace.
+
+Definition auxiliary_trace {Λ} (AS : AuxState Λ) := list (aux_state AS).
+
+Section auxiliary_trace.
+  Context `{AS : AuxState Λ}.
+
+  Definition singleton_auxtr (δ : aux_state AS) : auxiliary_trace AS := [δ].
+
+  Definition auxtr_starts_in
+             (atr : auxiliary_trace AS) (δ : aux_state AS) : Prop :=
+    hd_error atr = Some δ.
+
+  Definition auxtr_ends_in (atr : auxiliary_trace AS) (δ : aux_state AS)
+    : Prop := last atr = Some δ.
+
+  Lemma singleton_auxtr_starts_in δ : auxtr_starts_in (singleton_auxtr δ) δ.
+  Proof. done. Qed.
+
+  Lemma singleton_auxtr_ends_in δ : auxtr_ends_in (singleton_auxtr δ) δ.
+  Proof. done. Qed.
+
+  Lemma auxtr_ends_in_inj atr δ δ' :
+    auxtr_ends_in atr δ → auxtr_ends_in atr δ' → δ = δ'.
+  Proof. rewrite /auxtr_ends_in; intros ->; congruence. Qed.
+
+  Definition auxtr_extend (atr : auxiliary_trace AS) (δ : aux_state AS) :=
+    atr ++ [δ].
+
+  Definition auxtr_contract (atr atr' : auxiliary_trace AS) : Prop :=
+    ∃ δ, atr = auxtr_extend atr' δ.
+
+  Lemma auxtr_contract_of_extend atr δ atr' :
+    auxtr_contract (auxtr_extend atr δ) atr' → atr' = atr.
+  Proof. intros [? [? ?]%app_singleton_inv]; done. Qed.
+
+  Lemma auxtr_extend_starts_in atr δ' δ :
+    auxtr_starts_in atr δ' → auxtr_starts_in (auxtr_extend atr δ) δ'.
+  Proof.
+    rewrite /auxtr_starts_in /auxtr_extend /=; intros Hec'.
+    assert (atr = δ' :: tail atr) as -> by by apply hd_error_tl_repr.
+    done.
+  Qed.
+
+  Lemma auxtr_extend_ends_in atr δ : auxtr_ends_in (auxtr_extend atr δ) δ.
+  Proof. apply last_snoc. Qed.
+
+End auxiliary_trace.
+
+Section system_trace.
+  Context `(AS : AuxState Λ).
+
+  Inductive valid_system_trace : execution_trace Λ → auxiliary_trace AS → Prop :=
+  | valid_system_trace_singleton c δ :
+      valid_system_trace (singleton_exec c) (singleton_auxtr δ)
+  | valid_system_trace_step ex atr c κ c' δ δ' :
+      exec_ends_in ex c →
+      step c κ c' →
+      auxtr_ends_in atr δ →
+      valid_state_evolution AS c.2 δ κ c'.2 δ' →
+      valid_system_trace ex atr →
+      valid_system_trace (exec_extend ex κ c') (auxtr_extend atr δ').
+
+  Lemma valid_system_trace_valid_exec_trace ex atr :
+    valid_system_trace ex atr → valid_exec ex.
+  Proof. induction 1; econstructor; eauto. Qed.
+
+  Lemma valid_system_trace_singletons c δ :
+    valid_system_trace (singleton_exec c) (singleton_auxtr δ).
+  Proof. constructor. Qed.
+
+  Lemma valid_system_trace_extend ex atr c κ c' δ δ' :
+    valid_system_trace ex atr →
+    exec_ends_in ex c →
+    step c κ c' →
+    auxtr_ends_in atr δ →
+    valid_state_evolution AS c.2 δ κ c'.2 δ' →
+    valid_system_trace (exec_extend ex κ c') (auxtr_extend atr δ').
+  Proof.
+    intros Heatr; revert c κ c' δ δ'.
+    induction Heatr as [|? ? ? ? ? ? ? ? ? ? ? ? IHeatr]; intros c1 κ' c2.
+    - intros; econstructor; [done|done|done|done|constructor].
+    - intros; econstructor; [done|done|done|done|].
+      eapply IHeatr; eauto.
+  Qed.
+
+End system_trace.
